new/golang/theory/vmap.v
@@ -1,0 +1,22 @@
+From Perennial.goose_lang Require Import proofmode lifting.
+From New.golang.defn Require Export vmap.
+From New.golang.theory Require Import list.
+
+Section wps.
+Context `{sem: ffi_semantics} `{!ffi_interp ffi} `{!heapGS Σ}.
+
+(* XXX: this is a "pure" step. *)
+Lemma wp_vmap_Insert (k v : val) (m : gmap val val) :
+  {{{ True }}}
+    vmap.Insert k v (vmap.val m)
+  {{{ RET (vmap.val (<[k := v]> m)); True }}}
+.
+Proof.
+  iIntros (?) "_ HΦ".
+  rewrite vmap.val_unseal /vmap.Insert.
+  wp_pures.
+  rewrite /vmap.val_def.
+  iApply "HΦ".
+Qed.
+
+End wps.
